[[柯西函数方程]]在[[有理数]]域下的解：

已知：

$$
\forall x,y\in\mathbb{Q}, f(x+y)=f(x)+f(y)
$$

由 $f(0)=f(0)+f(0)$ 知 $f(0)=0$

$n=1$ 时显然$$f(n)=f(1)n$$成立，而

$$
\forall x\in\R,\forall n\in\N_{+},f((n+1)x)=f(x)+f(nx)
$$

由[[数学归纳法]]知 

$$
\forall x\in\R,\forall n\in\N_{+},f(nx)=f(x)n \tag{1}
$$

带入 $x=1$，即

$$
\forall n\in\N_{+},f(n)=f(1)n \tag{2}
$$

又

$$\forall n\in\N, f(n)+f(-n)=f(0)=0$$

即$f(-n)=-f(n)=f(1)\cdot(-1)$

故

$$\forall m\in\Z,f(m)=f(1)m \tag{3}$$
带入 $x=\frac{m}{n}$ 于(1)式，

$$\forall m\in\Z,\forall n\in\N_{+},f(m)=f\left(\frac{m}{n}\right)n$$

又由(3)式知

$$\forall m\in\Z,\forall n\in\N_{+},f\left(\frac{m}{n}\right)=\frac{1}{n}f(m)=\frac{m}{n}f(1)$$

即

$$\forall p\in\mathbb{Q},f(p)=f(1)p \tag{4}$$
